coq/D1Fold.v
@@ -82,6 +82,7 @@ Fixpoint replace_call (fn new_name : string) (body : p_expr) : p_expr :=
                              (replace_call fn new_name e2)
   | PListHead e => PListHead (replace_call fn new_name e)
   | PListTail e => PListTail (replace_call fn new_name e)
+  | PListIsNil e => PListIsNil (replace_call fn new_name e)
   | PCall f args =>
       let args' := map (replace_call fn new_name) args in
       if String.eqb f fn then PCall new_name args'
@@ -141,6 +142,7 @@ Fixpoint subst_expr (param : string) (arg : p_expr) (body : p_expr) : p_expr :=
       (if String.eqb x param then e2 else subst_expr param arg e2)
   | PListHead e => PListHead (subst_expr param arg e)
   | PListTail e => PListTail (subst_expr param arg e)
+  | PListIsNil e => PListIsNil (subst_expr param arg e)
   end.
 
 Fixpoint supercompile_d1
